Garden/OpenVM/Sha256/air_expr.v
@@ -1,0 +1,71 @@
+Require Import Garden.Plonky3.M.
+Require Import Garden.Plonky3.MExpr.
+Require Import Garden.OpenVM.Sha256.columns.
+Require Import Garden.OpenVM.Sha256.utils.
+
+(*
+fn eval_row<AB: InteractionBuilder>(&self, builder: &mut AB, start_col: usize)
+where
+    AB: LoggingAirBuilder,
+{
+    builder.log_in_constraints("eval_row");
+    let main = builder.main();
+    let local = main.row_slice(0);
+
+    // Doesn't matter which column struct we use here as we are only interested in the common
+    // columns
+    let local_cols: &Sha256DigestCols<AB::Var> =
+        local[start_col..start_col + SHA256_DIGEST_WIDTH].borrow();
+    let flags = &local_cols.flags;
+    builder.log_in_constraints("eval_row::flags");
+    builder.assert_bool(flags.is_round_row);
+    builder.assert_bool(flags.is_first_4_rows);
+    builder.assert_bool(flags.is_digest_row);
+    builder.assert_bool(flags.is_round_row + flags.is_digest_row);
+    builder.assert_bool(flags.is_last_block);
+
+    // Constrain a, e, being composed of bits: we make sure a and e are always in the same place
+    // in the trace matrix Note: this has to be true for every row, even padding rows
+    builder.log_in_constraints("eval_row::hash");
+    for i in 0..SHA256_ROUNDS_PER_ROW {
+        for j in 0..SHA256_WORD_BITS {
+            builder.assert_bool(local_cols.hash.a[i][j]);
+            builder.assert_bool(local_cols.hash.e[i][j]);
+        }
+    }
+}
+*)
+Definition eval_row (start_col : Z) (local_cols : Sha256DigestCols.t Var.t) : MExpr.t unit :=
+  msg! "eval_row" in
+  let flags := local_cols.(Sha256DigestCols.flags) in
+  msg! "eval_row::flags" in
+  let! _ := MExpr.assert_bool (Expr.Var flags.(Sha256FlagsCols.is_round_row)) in
+  let! _ := MExpr.assert_bool (Expr.Var flags.(Sha256FlagsCols.is_first_4_rows)) in
+  let! _ := MExpr.assert_bool (Expr.Var flags.(Sha256FlagsCols.is_digest_row)) in
+  let! _ := MExpr.assert_bool (
+    Expr.Add
+      (Expr.Var flags.(Sha256FlagsCols.is_round_row))
+      (Expr.Var flags.(Sha256FlagsCols.is_digest_row))
+  ) in
+  let! _ := MExpr.assert_bool (Expr.Var flags.(Sha256FlagsCols.is_last_block)) in
+  msg! "eval_row::hash" in
+  let! _ := for_in_zero_to_n SHA256_ROUNDS_PER_ROW (fun i =>
+    for_in_zero_to_n SHA256_WORD_BITS (fun j =>
+      let! _ := MExpr.assert_bool (Expr.Var local_cols.(Sha256DigestCols.hash).(Sha256WorkVarsCols.a).[i].[j]) in
+      let! _ := MExpr.assert_bool (Expr.Var local_cols.(Sha256DigestCols.hash).(Sha256WorkVarsCols.e).[i].[j]) in
+      MExpr.pure tt
+    )
+  ) in
+  MExpr.pure tt.
+
+Definition print_eval_row : string :=
+  let start_col := 0 in
+  let local_cols : Sha256DigestCols.t Var.t :=
+    MGenerateVar.eval MGenerateVar.generate in
+  ToRocq.cats [
+    ToRocq.endl;
+    ToRocq.to_rocq (eval_row start_col local_cols) 0;
+    ToRocq.endl
+  ].
+
+Compute print_eval_row.
