Garden/OpenVM/Sha256/columns.v
@@ -1,0 +1,146 @@
+Require Import Garden.Plonky3.M.
+Require Import Garden.Plonky3.MExpr.
+Require Import Garden.OpenVM.Sha256.utils.
+
+(*
+pub struct Sha256FlagsCols<T> {
+    pub is_round_row: T,
+    pub is_first_4_rows: T,
+    pub is_digest_row: T,
+    pub is_last_block: T,
+    pub row_idx: [T; SHA256_ROW_VAR_CNT],
+    pub global_block_idx: T,
+    pub local_block_idx: T,
+}
+*)
+Module Sha256FlagsCols.
+  Record t {T : Set} : Set := {
+    is_round_row : T;
+    is_first_4_rows : T;
+    is_digest_row : T;
+    is_last_block : T;
+    row_idx : Array.t T SHA256_ROW_VAR_CNT;
+    global_block_idx : T;
+    local_block_idx : T;
+  }.
+  Arguments t : clear implicits.
+
+  Definition map {T1 T2 : Set} (f : T1 -> T2) (self : t T1) : t T2 := {|
+    Sha256FlagsCols.is_round_row := f self.(Sha256FlagsCols.is_round_row);
+    Sha256FlagsCols.is_first_4_rows := f self.(Sha256FlagsCols.is_first_4_rows);
+    Sha256FlagsCols.is_digest_row := f self.(Sha256FlagsCols.is_digest_row);
+    Sha256FlagsCols.is_last_block := f self.(Sha256FlagsCols.is_last_block);
+    Sha256FlagsCols.row_idx := Array.map f self.(Sha256FlagsCols.row_idx);
+    Sha256FlagsCols.global_block_idx := f self.(Sha256FlagsCols.global_block_idx);
+    Sha256FlagsCols.local_block_idx := f self.(Sha256FlagsCols.local_block_idx);
+  |}.
+
+  Global Instance IsGenerateVar : MGenerateVar.C (t Var.t) := {
+    generate :=
+      [[
+        {|
+          Sha256FlagsCols.is_round_row := MGenerateVar.generate (||);
+          Sha256FlagsCols.is_first_4_rows := MGenerateVar.generate (||);
+          Sha256FlagsCols.is_digest_row := MGenerateVar.generate (||);
+          Sha256FlagsCols.is_last_block := MGenerateVar.generate (||);
+          Sha256FlagsCols.row_idx := MGenerateVar.generate (||);
+          Sha256FlagsCols.global_block_idx := MGenerateVar.generate (||);
+          Sha256FlagsCols.local_block_idx := MGenerateVar.generate (||);
+        |}
+      ]];
+  }.
+End Sha256FlagsCols.
+
+(*
+pub struct Sha256WorkVarsCols<T> {
+    /// `a` and `e` after each iteration as 32-bits
+    pub a: [[T; SHA256_WORD_BITS]; SHA256_ROUNDS_PER_ROW],
+    pub e: [[T; SHA256_WORD_BITS]; SHA256_ROUNDS_PER_ROW],
+    /// The carry's used for addition during each iteration when computing `a` and `e`
+    pub carry_a: [[T; SHA256_WORD_U16S]; SHA256_ROUNDS_PER_ROW],
+    pub carry_e: [[T; SHA256_WORD_U16S]; SHA256_ROUNDS_PER_ROW],
+}
+*)
+Module Sha256WorkVarsCols.
+  Record t {T : Set} : Set := {
+    a : Array.t (Array.t T SHA256_WORD_BITS) SHA256_ROUNDS_PER_ROW;
+    e : Array.t (Array.t T SHA256_WORD_BITS) SHA256_ROUNDS_PER_ROW;
+    carry_a : Array.t (Array.t T SHA256_WORD_U16S) SHA256_ROUNDS_PER_ROW;
+    carry_e : Array.t (Array.t T SHA256_WORD_U16S) SHA256_ROUNDS_PER_ROW;
+  }.
+  Arguments t : clear implicits.
+
+  Global Instance IsGenerateVar : MGenerateVar.C (t Var.t) := {
+    generate :=
+      [[
+        {|
+          Sha256WorkVarsCols.a := MGenerateVar.generate (||);
+          Sha256WorkVarsCols.e := MGenerateVar.generate (||);
+          Sha256WorkVarsCols.carry_a := MGenerateVar.generate (||);
+          Sha256WorkVarsCols.carry_e := MGenerateVar.generate (||);
+        |}
+      ]];
+  }.
+End Sha256WorkVarsCols.
+
+(*
+pub struct Sha256MessageHelperCols<T> {
+    pub w_3: [[T; SHA256_WORD_U16S]; SHA256_ROUNDS_PER_ROW - 1],
+    pub intermed_4: [[T; SHA256_WORD_U16S]; SHA256_ROUNDS_PER_ROW],
+    pub intermed_8: [[T; SHA256_WORD_U16S]; SHA256_ROUNDS_PER_ROW],
+    pub intermed_12: [[T; SHA256_WORD_U16S]; SHA256_ROUNDS_PER_ROW],
+}
+*)
+Module Sha256MessageHelperCols.
+  Record t {T : Set} : Set := {
+    w_3 : Array.t (Array.t T SHA256_WORD_U16S) (SHA256_ROUNDS_PER_ROW - 1);
+    intermed_4 : Array.t (Array.t T SHA256_WORD_U16S) SHA256_ROUNDS_PER_ROW;
+    intermed_8 : Array.t (Array.t T SHA256_WORD_U16S) SHA256_ROUNDS_PER_ROW;
+    intermed_12 : Array.t (Array.t T SHA256_WORD_U16S) SHA256_ROUNDS_PER_ROW;
+  }.
+  Arguments t : clear implicits.
+
+  Global Instance IsGenerateVar : MGenerateVar.C (t Var.t) := {
+    generate :=
+      [[
+        {|
+          Sha256MessageHelperCols.w_3 := MGenerateVar.generate (||);
+          Sha256MessageHelperCols.intermed_4 := MGenerateVar.generate (||);
+          Sha256MessageHelperCols.intermed_8 := MGenerateVar.generate (||);
+          Sha256MessageHelperCols.intermed_12 := MGenerateVar.generate (||);
+        |}
+      ]];
+  }.
+End Sha256MessageHelperCols.
+(*
+pub struct Sha256DigestCols<T> {
+    pub flags: Sha256FlagsCols<T>,
+    pub hash: Sha256WorkVarsCols<T>,
+    pub schedule_helper: Sha256MessageHelperCols<T>,
+    pub final_hash: [[T; SHA256_WORD_U8S]; SHA256_HASH_WORDS],
+    pub prev_hash: [[T; SHA256_WORD_U16S]; SHA256_HASH_WORDS],
+}
+*)
+Module Sha256DigestCols.
+  Record t {T : Set} : Set := {
+    flags : Sha256FlagsCols.t T;
+    hash : Sha256WorkVarsCols.t T;
+    schedule_helper : Sha256MessageHelperCols.t T;
+    final_hash : Array.t (Array.t T SHA256_WORD_U8S) SHA256_HASH_WORDS;
+    prev_hash : Array.t (Array.t T SHA256_WORD_U16S) SHA256_HASH_WORDS;
+  }.
+  Arguments t : clear implicits.
+
+  Global Instance IsGenerateVar : MGenerateVar.C (t Var.t) := {
+    generate :=
+      [[
+        {|
+          Sha256DigestCols.flags := MGenerateVar.generate (||);
+          Sha256DigestCols.hash := MGenerateVar.generate (||);
+          Sha256DigestCols.schedule_helper := MGenerateVar.generate (||);
+          Sha256DigestCols.final_hash := MGenerateVar.generate (||);
+          Sha256DigestCols.prev_hash := MGenerateVar.generate (||);
+        |}
+      ]];
+  }.
+End Sha256DigestCols.
