Garden/OpenVM/primitives/encoder.v
@@ -1,0 +1,21 @@
+Require Import Garden.Plonky3.M.
+Require Import Garden.Plonky3.MExpr.
+
+(*
+pub struct Encoder {
+    var_cnt: usize,
+    flag_cnt: usize,
+    max_flag_degree: u32,
+    pts: Vec<Vec<u32>>,
+    reserve_invalid: bool,
+}
+*)
+Module Encoder.
+  Record t : Set := {
+    var_cnt : Z;
+    flag_cnt : Z;
+    max_flag_degree : Z;
+    pts : list (list Z);
+    reserve_invalid : bool;
+  }.
+End Encoder.
